Fix canonicity definition (#104)
* More opaque operators

* Fix

* Fix canonicity

* More fixes

* More

* Try

* Switch

* Fix, compiled

* Fixes

* Restore

* More fix

* More

* Fix CpcMini

* Fix substitution default

* Refactor

* More

* More

* More

* Minor, refactored

* Fixes to rules

Cpc/SmtModel.lean
@@ -1728,7 +1728,9 @@ def __smtx_typeof : SmtTerm -> SmtType
   | (SmtTerm.bvusubo x1 x2) => (__smtx_typeof_bv_op_2_ret (__smtx_typeof x1) (__smtx_typeof x2) SmtType.Bool)
   | (SmtTerm.bvssubo x1 x2) => (__smtx_typeof_bv_op_2_ret (__smtx_typeof x1) (__smtx_typeof x2) SmtType.Bool)
   | (SmtTerm.bvsdivo x1 x2) => (__smtx_typeof_bv_op_2_ret (__smtx_typeof x1) (__smtx_typeof x2) SmtType.Bool)
-  | (SmtTerm.seq_empty x1) => (__smtx_typeof_guard_wf x1 (SmtType.Seq x1))
+  | (SmtTerm.seq_empty x1) => 
+    let _v0 := (SmtType.Seq x1)
+    (__smtx_typeof_guard_wf _v0 _v0)
   | (SmtTerm.str_len x1) => (__smtx_typeof_seq_op_1_ret (__smtx_typeof x1) SmtType.Int)
   | (SmtTerm.str_concat x1 x2) => (__smtx_typeof_seq_op_2 (__smtx_typeof x1) (__smtx_typeof x2))
   | (SmtTerm.str_substr x1 x2 x3) => (__smtx_typeof_str_substr (__smtx_typeof x1) (__smtx_typeof x2) (__smtx_typeof x3))
@@ -1788,13 +1790,15 @@ def __smtx_typeof : SmtTerm -> SmtType
   | (SmtTerm.re_loop x1 x2 x3) => (__smtx_typeof_re_loop x1 x2 (__smtx_typeof x3))
   | (SmtTerm.str_in_re x1 x2) => (native_ite (native_Teq (__smtx_typeof x1) (SmtType.Seq SmtType.Char)) (native_ite (native_Teq (__smtx_typeof x2) SmtType.RegLan) SmtType.Bool SmtType.None) SmtType.None)
   | (SmtTerm.seq_unit x1) => 
-    let _v0 := (__smtx_typeof x1)
-    (__smtx_typeof_guard_wf _v0 (SmtType.Seq _v0))
+    let _v0 := (SmtType.Seq (__smtx_typeof x1))
+    (__smtx_typeof_guard_wf _v0 _v0)
   | (SmtTerm.seq_nth x1 x2) => (__smtx_typeof_seq_nth (__smtx_typeof x1) (__smtx_typeof x2))
-  | (SmtTerm.set_empty x1) => (__smtx_typeof_guard_wf x1 (SmtType.Set x1))
+  | (SmtTerm.set_empty x1) => 
+    let _v0 := (SmtType.Set x1)
+    (__smtx_typeof_guard_wf _v0 _v0)
   | (SmtTerm.set_singleton x1) => 
-    let _v0 := (__smtx_typeof x1)
-    (__smtx_typeof_guard_wf _v0 (SmtType.Set _v0))
+    let _v0 := (SmtType.Set (__smtx_typeof x1))
+    (__smtx_typeof_guard_wf _v0 _v0)
   | (SmtTerm.set_union x1 x2) => (__smtx_typeof_sets_op_2 (__smtx_typeof x1) (__smtx_typeof x2))
   | (SmtTerm.set_inter x1 x2) => (__smtx_typeof_sets_op_2 (__smtx_typeof x1) (__smtx_typeof x2))
   | (SmtTerm.set_minus x1 x2) => (__smtx_typeof_sets_op_2 (__smtx_typeof x1) (__smtx_typeof x2))
@@ -1825,7 +1829,7 @@ def __smtx_typeof : SmtTerm -> SmtType
 
 def __smtx_is_unit_datatype_cons : SmtDatatypeCons -> native_Bool
   | SmtDatatypeCons.unit => true
-  | (SmtDatatypeCons.cons T c) => (native_and (smtx_is_unit_type T) (__smtx_is_unit_datatype_cons c))
+  | (SmtDatatypeCons.cons T c) => (native_and (__smtx_is_unit_type T) (__smtx_is_unit_datatype_cons c))
 
 
 def __smtx_is_unit_datatype : SmtDatatype -> native_Bool
@@ -1833,43 +1837,73 @@ def __smtx_is_unit_datatype : SmtDatatype -> native_Bool
   | d => false
 
 
-def smtx_is_unit_type : SmtType -> native_Bool
+def __smtx_is_unit_type : SmtType -> native_Bool
   | (SmtType.BitVec w) => (native_nateq w native_nat_zero)
   | (SmtType.Datatype s d) => (__smtx_is_unit_datatype d)
-  | (SmtType.Map T U) => (smtx_is_unit_type U)
-  | (SmtType.FunType T U) => (smtx_is_unit_type U)
+  | (SmtType.Map T U) => (__smtx_is_unit_type U)
+  | (SmtType.FunType T U) => (__smtx_is_unit_type U)
   | T => false
 
 
-def __smtx_finite_datatype_cons_default (v : SmtValue) : SmtDatatypeCons -> SmtValue
+def __smtx_is_finite_datatype_cons : SmtDatatypeCons -> native_Bool
+  | SmtDatatypeCons.unit => true
+  | (SmtDatatypeCons.cons T c) => (native_and (__smtx_is_finite_type T) (__smtx_is_finite_datatype_cons c))
+
+
+def __smtx_is_finite_datatype : SmtDatatype -> native_Bool
+  | SmtDatatype.null => true
+  | (SmtDatatype.sum c d) => (native_and (__smtx_is_finite_datatype_cons c) (__smtx_is_finite_datatype d))
+
+
+def __smtx_is_finite_type : SmtType -> native_Bool
+  | SmtType.Bool => true
+  | (SmtType.BitVec w) => true
+  | SmtType.Char => true
+  | (SmtType.Datatype s d) => (__smtx_is_finite_datatype d)
+  | (SmtType.Map T U) => (native_or (__smtx_is_unit_type U) (native_and (__smtx_is_finite_type T) (__smtx_is_finite_type U)))
+  | (SmtType.FunType T U) => (native_or (__smtx_is_unit_type U) (native_and (__smtx_is_finite_type T) (__smtx_is_finite_type U)))
+  | (SmtType.Set T) => (__smtx_is_finite_type T)
+  | (SmtType.Seq T) => (__smtx_is_finite_type T)
+  | T => false
+
+
+def __smtx_value_dt_substitute_apply (s : native_String) (v1 : SmtValue) (v2 : SmtValue) : SmtValue -> SmtValue
+  | (SmtValue.DtCons s2 d i) => (native_ite (native_streq s s2) v1 v2)
+  | v => v2
+
+
+def __smtx_value_dt_substitute (s : native_String) (d : SmtDatatype) : SmtValue -> SmtValue
+  | (SmtValue.DtCons s2 d2 i) => (SmtValue.DtCons s2 (native_ite (native_streq s s2) d2 (__smtx_dt_substitute s d d2)) i)
+  | (SmtValue.Apply f v) => (__smtx_value_dt_substitute_apply s (SmtValue.Apply f v) (SmtValue.Apply (__smtx_value_dt_substitute s d f) (__smtx_value_dt_substitute s d v)) (__vsm_apply_head f))
+  | v => v
+
+
+def __smtx_datatype_cons_default (s : native_String) (d : SmtDatatype) (v : SmtValue) : SmtDatatypeCons -> SmtValue
   | SmtDatatypeCons.unit => v
   | (SmtDatatypeCons.cons T c) => 
-    let _v0 := (__smtx_finite_type_default T)
-    (native_ite (native_veq _v0 SmtValue.NotValue) SmtValue.NotValue (__smtx_finite_datatype_cons_default (SmtValue.Apply v _v0) c))
+    let _v0 := (__smtx_value_dt_substitute s d (__smtx_type_default T))
+    (native_ite (native_veq _v0 SmtValue.NotValue) SmtValue.NotValue (__smtx_datatype_cons_default s d (SmtValue.Apply v _v0) c))
 
 
-def __smtx_finite_datatype_default (s : native_String) (d0 : SmtDatatype) : SmtDatatype -> native_Nat -> SmtValue
+def __smtx_datatype_default (s : native_String) (d0 : SmtDatatype) : SmtDatatype -> native_Nat -> SmtValue
   | SmtDatatype.null, n => SmtValue.NotValue
-  | (SmtDatatype.sum c SmtDatatype.null), n => (__smtx_finite_datatype_cons_default (SmtValue.DtCons s d0 n) c)
   | (SmtDatatype.sum c d), n => 
-    let _v0 := (__smtx_finite_datatype_cons_default (SmtValue.DtCons s d0 n) c)
-    (native_ite (native_and (native_not (native_veq _v0 SmtValue.NotValue)) (native_not (native_veq (__smtx_finite_datatype_default s d0 d (native_nat_succ n)) SmtValue.NotValue))) _v0 SmtValue.NotValue)
+    let _v0 := (__smtx_datatype_cons_default s d0 (SmtValue.DtCons s d0 n) c)
+    (native_ite (native_not (native_veq _v0 SmtValue.NotValue)) _v0 (__smtx_datatype_default s d0 d (native_nat_succ n)))
 
 
-def __smtx_finite_type_default : SmtType -> SmtValue
+def __smtx_type_default : SmtType -> SmtValue
   | SmtType.Bool => (SmtValue.Boolean false)
+  | SmtType.Int => (SmtValue.Numeral 0)
+  | SmtType.Real => (SmtValue.Rational (native_mk_rational 0 1))
   | (SmtType.BitVec w) => (SmtValue.Binary (native_nat_to_int w) 0)
   | SmtType.Char => (SmtValue.Char (native_nat_to_char native_nat_zero))
-  | (SmtType.Datatype s d) => (__smtx_finite_datatype_default s d d native_nat_zero)
-  | (SmtType.Map T U) => 
-    let _v0 := (__smtx_finite_type_default U)
-    let _v1 := (SmtValue.Map (SmtMap.default T _v0))
-    (native_ite (smtx_is_unit_type U) _v1 (native_ite (native_and (native_not (native_veq (__smtx_finite_type_default T) SmtValue.NotValue)) (native_not (native_veq _v0 SmtValue.NotValue))) _v1 SmtValue.NotValue))
-  | (SmtType.Set T) => (native_ite (native_veq (__smtx_finite_type_default T) SmtValue.NotValue) SmtValue.NotValue (SmtValue.Set (SmtMap.default T (SmtValue.Boolean false))))
-  | (SmtType.FunType T U) => 
-    let _v0 := (__smtx_finite_type_default U)
-    let _v1 := (SmtValue.Fun (SmtMap.default T _v0))
-    (native_ite (smtx_is_unit_type U) _v1 (native_ite (native_and (native_not (native_veq (__smtx_finite_type_default T) SmtValue.NotValue)) (native_not (native_veq _v0 SmtValue.NotValue))) _v1 SmtValue.NotValue))
+  | (SmtType.Datatype s d) => (__smtx_datatype_default s d d native_nat_zero)
+  | (SmtType.Map T U) => (SmtValue.Map (SmtMap.default T (__smtx_type_default U)))
+  | (SmtType.Set T) => (SmtValue.Set (SmtMap.default T (SmtValue.Boolean false)))
+  | (SmtType.Seq T) => (SmtValue.Seq (SmtSeq.empty T))
+  | (SmtType.USort i) => (SmtValue.UValue i native_nat_zero)
+  | (SmtType.FunType T U) => (SmtValue.Fun (SmtMap.default T (__smtx_type_default U)))
   | T => SmtValue.NotValue
 
 
@@ -1879,9 +1913,7 @@ def __smtx_map_entries_ordered_after (i : SmtValue) : SmtMap -> native_Bool
 
 
 def __smtx_map_default_canonical (T : SmtType) (e : SmtValue) : native_Bool :=
-  
-    let _v0 := (__smtx_typeof_value e)
-    (native_ite (native_veq (__smtx_finite_type_default (SmtType.Map T _v0)) SmtValue.NotValue) true (native_veq e (__smtx_finite_type_default _v0)))
+  (native_ite (__smtx_is_finite_type T) (native_veq e (__smtx_type_default (__smtx_typeof_value e))) true)
 
 def __smtx_map_canonical : SmtMap -> native_Bool
   | (SmtMap.default T e) => (native_and (__smtx_map_default_canonical T e) (__smtx_value_canonical_bool e))
@@ -2219,9 +2251,9 @@ def __smtx_value_canonical (v : SmtValue) : Prop :=
   __smtx_value_canonical_bool v = true
 
 def model_total_typed (M : SmtModel) : Prop :=
-  (∀ s T, type_inhabited T -> __smtx_typeof_value (__smtx_model_lookup M s T) = T) ∧
-  (∀ s T, type_inhabited T -> __smtx_value_canonical (__smtx_model_lookup M s T)) ∧
-  (∀ s T, ¬ type_inhabited T -> __smtx_model_lookup M s T = SmtValue.NotValue)
+  (∀ s T, __smtx_type_wf T = true -> __smtx_typeof_value (__smtx_model_lookup M s T) = T) ∧
+  (∀ s T, __smtx_type_wf T = true -> __smtx_value_canonical (__smtx_model_lookup M s T)) ∧
+  (∀ s T, __smtx_type_wf T = false -> __smtx_model_lookup M s T = SmtValue.NotValue)
 
 /-
 SMT interpretation is satisfiability, i.e. the existence of a model
